Move ata type definitions to [eval_rules]

coq-osiris/examples/proofs/splay.v
@@ -109,108 +109,6 @@ Definition zlt {A} (z1 z2 : zipper A) :=
   {| wf_relation := zlt |}.
 Next Obligation. constructor; unfold zlt; apply wf_inverse_image, lt_wf. Qed.
 
-(* -------------------------------------------------------------------------- *)
-
-(* Fun with data constructors: we can know the destructor as long as we
-   have the signature of the algebraic datatype. *)
-
-(* The type of a data constructor can be built from the list of
-   constructor argument types. *)
-Fixpoint data_constructor A (x : list Type) : Type :=
-  match x with
-    | nil => A
-    | hd :: tl => hd -> data_constructor A tl
-  end.
-
-(* A signature for a constructor that builds type [A]. *)
-Definition signature {A} : Type := sigT (data_constructor A).
-
-(* Data types is a map from string (constructor name) to the type signatures
-  of the constructors. *)
-Class DataType (A : Type) :=
-  { data_signature : gmap string (@signature A); }.
-
-(* -------------------------------------------------------------------------- *)
-
-Set Implicit Arguments.
-
-(* Heterogeneous list *)
-
-Inductive hlist (A : Type) (B : A -> Type) : list A -> Type :=
-| HNil : hlist B nil
-| HCons : forall (x : A) (ls : list A), B x -> hlist B ls -> hlist B (x :: ls).
-Arguments HNil {A B}.
-Arguments HCons {A B x ls}.
-
-From Equations Require Import Equations.
-
-(* Append for heterogeneous lists. *)
-
-Equations happ (A B : list Type) :
-  hlist (fun T : Type => T) A ->
-  hlist (fun T : Type => T) B ->
-  hlist (fun T : Type => T) (A ++ B) :=
-happ HNil m := m;
-happ (HCons a l1) m := HCons a (happ l1 m).
-
-(* -------------------------------------------------------------------------- *)
-
-(* Construct a data type [A] given its signature, data constructor and arguments. *)
-
-Equations build_constructor {A}
-  (Σ : list Type)
-  (constr : data_constructor A Σ)
-  (data : hlist (fun T : Type => T) Σ)
-  : A :=
-  (* When there are no arguments left, the construction is immediate. *)
-  @build_constructor _ nil constr HNil := constr;
-
-  (* Peel off an argument of the signature and apply to the constructor. *)
-  @build_constructor _ (τ :: tl) constr (HCons v vtl) :=
-    (build_constructor (Σ := tl) (constr v) vtl).
-
-(* TODO Comment *)
-
-Fixpoint eval_data_aux {A X}
-  (v : list expr)
-  (η : env)
-  (φ : A -> Prop) (ψ : exn -> Prop)
-  (t : list Type)
-  (constr : data_constructor A X)
-  (acc_t : list Type)
-  (acc : hlist (fun T : Type => T) acc_t)
-  : Prop :=
-  match v, t with
-  | hd :: tl, hd_t :: tl_t =>
-      ∃ (EncX : Encode hd_t) x,
-      pure
-        (eval η hd)
-        (fun y : hd_t =>
-          y = x /\
-          @eval_data_aux _ _ tl η φ ψ
-            tl_t
-            constr
-            (acc_t ++ [hd_t])
-            (happ acc (HCons x HNil))) ψ
-  | nil, nil =>
-      exists (eq_X : acc_t = X),
-      φ (@build_constructor _ acc_t
-           (eq_rect_r
-              (fun X => data_constructor A X)
-              constr eq_X) acc)
-  | _ , _ => False
-end.
-
-Arguments eval_data_aux {A X} _ _ _ _ _ _ _ _.
-
-(* Evaluate a list of expressions into a data type according to the signature. *)
-
-Definition eval_data {A}
-  (e : list expr) (η : env) (φ : A -> Prop) (ψ : exn -> Prop) (Σ : @splay.signature A)
-  := @eval_data_aux A _ e η φ ψ (projT1 Σ) (projT2 Σ) nil HNil.
-
-(* -------------------------------------------------------------------------- *)
-
 (* Datatype instance for [tree] *)
 
 (* LATER: Can this be generated during translation? *)
@@ -344,44 +242,17 @@ Section splay_proofs.
 
 (* -------------------------------------------------------------------------- *)
 
-(* TODO : Move and prove. *)
-Lemma pure_eval_data {A} `{Encode A, DataType A} η
-  c hd tl (φ : _ -> Prop) ψ
-  (signature : sigT (data_constructor A)) :
-  data_signature !! c = Some signature ->
-  eval_data (hd :: tl) η φ ψ signature ->
-  pure (A := A) (eval η (EData c (hd :: tl))) φ ψ.
-Proof. Admitted.
-
-(* TODO: Tweak this definition. *)
-Lemma total_ret_eq_and `{Encode A} {X : Type} (a : A) (ψ : Prop):
-  ψ →
-  total (E := X) (ret #a) (λ a', a' = a /\ ψ).
-Proof.
-  intros. eapply total_mono. apply total_ret_eq.
-  cbn. intros; by subst.
-Qed.
-
-Ltac pure_eval_path :=
-  eexists _, _;
-  eapply pure_eval_path, total_ret_eq_and.
-Ltac pure_data :=
-  eapply pure_eval_data;
-  first try done;
-  repeat pure_eval_path; exists eq_refl.
-
-(* -------------------------------------------------------------------------- *)
-
 Lemma Splay_spec :
   splay_spec
     (VCloRec stdlib_env [RecBinding "splay" (AnonFunction __branches1)] "splay").
 Proof.
   intros A H ctx l x r.
 
-  (* We need to massage the postcondition so we can generalize the argument for the
-     recursive call. *)
+  (* We need to massage the postcondition so we can generalize the argument for
+    the recursive call. *)
   change (λ t', fringe t' = fringe (fill ctx (Node l x r))) with
-    ((λ '(l, x, r, ctx) t', fringe t' = fringe (fill ctx (Node l x r))) (l, x, r, ctx)).
+    ((λ '(l, x, r, ctx) t', fringe t' = fringe (fill ctx (Node l x r)))
+         (l, x, r, ctx)).
 
   (* Recursion, with decreasing depth of zipper. *)
   recursion { measure snd } ∀ (l, x, r, ctx).
@@ -396,10 +267,11 @@ Proof.
 
   destruct ctx eqn: Hctx.
   { (* Case: [ctx] matches [Root] *)
-    pure_match. pure_data.
-    prove_same_fringe. }
+    pure_match. pure_data. prove_same_fringe. }
 
   (* TODO: Generate custom match cases like before *)
+
+  (* We should be able to continually apply [pure_match_cons]. *)
 Admitted.
 
 Lemma Splay_leaf_spec splay :
